\begin{equation}
\mathbf{X}(u, t, s)=\sum_{i=0}^{m} \sum_{j=0}^{n} \sum_{k=0}^{p} \mathbf{a}^{(i, j, k)} f_{i}^{m}(u) g_{j}^{n}(t) h_{k}^{p}(s)
\label{ffd_3d}
\end{equation}
where Bernstein's polynomial $f_{i}^{m}(u)$ is defined as,

\begin{equation}
f_{i}^{m}(u)=\frac{(m) !}{(i) !(m-i) !} u^{i}(1-u)^{m-i}
\label{bernstein_poly}
\end{equation}

The new position of a point $\textbf{X}_{def}$ is computed by:

\begin{equation*}
\mathbf{X}_{d e f}=\sum_{i=0}^{l}\left(\begin{array}{l}
l \\
i
\end{array}\right)(1-s)^{l-i} s^{i}\left[\sum_{j=0}^{m}\left(\begin{array}{c}
m \\
j
\end{array}\right)(1-t)^{m-j} t^{j}\left(\sum_{k=0}^{n}\left(\begin{array}{l}
n \\
k
\end{array}\right)(1-u)^{n-k} u^{k} \mathbf{P}_{i j k}\right)\right]\end{equation*}